come cleanup (leaving 2 admits in tagged state, that are (probably) related to the split predicate not yet adapted to the new state predicate)

src/core/DY.Core.Trace.Invariant.fst
@@ -27,35 +27,54 @@ open DY.Core.Trace.Type
 /// This property will then be an essential ingredient of the attacker knowledge theorem
 /// (see DY.Core.Attacker.Knowledge.attacker_only_knows_publishable_values),
 /// to ensure that the every bytestring obtained by the attacker by corruption are publishable.
+///
+/// The state of a principal consists of three levels:
+/// * the **full state** of a principal consists of several **sessions**,
+///   which are identified by a state_id
+/// * a session is a chronologically ordered collection of **states**
+///
+/// In the state predicate, we can define predicates on all state levels.
+/// All predicates give conditions on when a new state can be added.
+/// 
+/// For example:
+/// consider a state consisting of
+/// (a nonce, a counter, a user_id).
+/// We could define the following predicates
+/// * the nonce must be knowable to the storing principal (this is a predicate on a single state `pred`)
+/// * the counter must increase within a session (this is a session predicate `session_pred`)
+/// * the user_id must be unique across different sessions (this is a predicate on the full state `full_state_pred`)
 
 noeq
 type state_predicate (cinvs:crypto_invariants) = {
-  pred: trace -> principal -> state_id -> bytes -> prop;
+  // the three predicates for adding a new state
+  pred: trace -> principal -> state_id -> state_raw -> prop;
+  session_pred: trace -> session_raw -> principal -> state_id -> state_raw -> prop; // the session argument is the current session on the trace
+  full_state_pred: trace -> full_state_raw -> principal -> state_id -> state_raw -> prop; // the full_state argument is the current full state on the trace
 
-  session_pred: trace -> session_raw -> principal -> state_id -> state_raw -> prop;
-  full_state_pred: trace -> full_state_raw -> principal -> state_id -> state_raw -> prop;
-
-  // TODO: Do we want the later lemma?
-  pred_later:
-    tr1:trace -> tr2:trace ->
-    prin:principal -> sess_id:state_id -> content:bytes ->
-    Lemma
-    (requires pred tr1 prin sess_id content /\ tr1 <$ tr2)
-    (ensures pred tr2 prin sess_id content)
-  ;
+  // for single states, we enforce that the stored content is knowable to the storing principal
   pred_knowable:
     tr:trace ->
-    prin:principal -> sess_id:state_id -> content:bytes ->
+    prin:principal -> sess_id:state_id -> content:state_raw ->
     Lemma
     (requires pred tr prin sess_id content)
     (ensures
       is_knowable_by #cinvs (L.principal_state_label prin sess_id) tr content
     )
   ;
-
+  
+  // the predicate for single states must stay true if the trace grows
+  pred_later:
+    tr1:trace -> tr2:trace ->
+    prin:principal -> sess_id:state_id -> content:state_raw ->
+    Lemma
+    (requires tr1 <$ tr2 /\ pred tr1 prin sess_id content)
+    (ensures pred tr2 prin sess_id content)
+  ;
+  // the session predicate must stay true, 
+  // if the trace grows but the session stays the same
   session_pred_grows: 
     tr1:trace -> tr2:trace -> 
-    sess:session_raw -> prin:principal -> sess_id:state_id -> content:bytes ->
+    sess:session_raw -> prin:principal -> sess_id:state_id -> content:state_raw ->
     Lemma
       (requires
         tr1 <$ tr2 /\ session_pred tr1 sess prin sess_id content
@@ -65,6 +84,10 @@ type state_predicate (cinvs:crypto_invariants) = {
       )
 }
 
+/// the predicates on the three state levels are combined to a `global_state_pred`
+
+// convenience functions lifting the session and full state predicates to `option`
+// (no restriction for `None`)
 val session_pred_: {|cinvs: crypto_invariants|} -> {|sp:state_predicate cinvs|} -> trace -> option session_raw -> principal -> state_id -> state_raw -> prop
 let session_pred_ #cinvs #sp  tr session prin sid content =
   match session with
@@ -77,15 +100,36 @@ let full_state_pred_ #cinvs #sp tr full_state prin sid content =
   | None -> True
   | Some full_st -> sp.full_state_pred tr full_st prin sid content
 
+/// the global state pred reads the current session and full state from the trace
+/// and uses those as arguments for the corresponding predicates
 
 val global_state_pred_: {|cinvs: crypto_invariants|} -> {|sp: state_predicate cinvs |} -> trace -> principal -> state_id -> state_raw -> prop
 let global_state_pred_ #cinvs #sp tr prin sid content =
   let session = get_session prin sid tr in
   let full_state = get_full_state prin tr in
-          sp.pred tr prin sid content
-        /\ session_pred_ tr session prin sid content
-        /\ full_state_pred_ tr full_state prin sid content 
+    sp.pred tr prin sid content
+  /\ session_pred_ tr session prin sid content
+  /\ full_state_pred_ tr full_state prin sid content 
 
+
+/// the session predicate remains true
+/// if the trace grows
+/// but there are no more state entries for the principal and the session
+
+val session_pred_later_:
+  {|cinvs: crypto_invariants |} -> {|sp:state_predicate cinvs |} ->
+  tr1:trace -> tr2:trace  -> p:principal -> sid:state_id -> cont:state_raw ->
+  Lemma
+    (requires 
+        tr1 <$ tr2 
+      /\ no_set_state_entry_for p sid (tr2 `suffix_after` tr1)
+      /\ sp.session_pred tr1 (get_session_aux p sid tr1) p sid cont
+    )
+    (ensures sp.session_pred tr2 (get_session_aux p sid tr2) p sid cont)
+let session_pred_later_ #_ #sp tr1 tr2 p sid cont =
+  get_session_aux_same p sid tr1 tr2;
+  let session = get_session_aux p sid tr1 in
+  sp.session_pred_grows tr1 tr2 session p sid cont
 
 /// The parameters of the trace invariant.
 
@@ -113,29 +157,16 @@ class protocol_invariants = {
 let state_pred {|invs:protocol_invariants|} = invs.trace_invs.state_pred.pred
 let session_pred {|invs:protocol_invariants|} = invs.trace_invs.state_pred.session_pred
 let full_state_pred {|invs:protocol_invariants|} = invs.trace_invs.state_pred.full_state_pred
-let state_pred_later {|invs:protocol_invariants|} = invs.trace_invs.state_pred.pred_later
 let state_pred_knowable {|invs:protocol_invariants|} = invs.trace_invs.state_pred.pred_knowable
+let state_pred_later {|invs:protocol_invariants|} = invs.trace_invs.state_pred.pred_later
 let session_pred_grows {|invs:protocol_invariants|} = invs.trace_invs.state_pred.session_pred_grows
-let global_state_pred {|invs:protocol_invariants|} = global_state_pred_ #invs.crypto_invs #invs.trace_invs.state_pred
 let session_pred_opt {|invs:protocol_invariants|} = session_pred_ #_ #invs.trace_invs.state_pred
 let full_state_pred_opt {|invs:protocol_invariants|} = full_state_pred_ #_ #invs.trace_invs.state_pred
+let global_state_pred {|invs:protocol_invariants|} = global_state_pred_ #invs.crypto_invs #invs.trace_invs.state_pred
+let session_pred_later {|invs:protocol_invariants|} = session_pred_later_ #invs.crypto_invs #invs.trace_invs.state_pred
 let event_pred {|invs:protocol_invariants|} = invs.trace_invs.event_pred
 
 
-val session_pred_later:
-{|protocol_invariants |} ->
-  tr1:trace -> tr2:trace  -> p:principal -> sid:state_id -> cont:state_raw ->
-  Lemma
-    (requires 
-        tr1 <$ tr2 
-      /\ no_set_state_entry_for p sid (tr2 `suffix_after` tr1)
-      /\ session_pred tr1 (get_session_aux p sid tr1) p sid cont
-    )
-    (ensures session_pred tr2 (get_session_aux p sid tr2) p sid cont)
-let session_pred_later tr1 tr2 p sid cont =
-  get_session_aux_same p sid tr1 tr2;
-  let session = get_session_aux p sid tr1 in
-  session_pred_grows tr1 tr2 session p sid cont
 
 (*** Trace invariant definition ***)
 
@@ -171,7 +202,28 @@ let rec trace_invariant #invs tr =
     trace_event_invariant tr_init event /\
     trace_invariant tr_init
 
+
+
 (*** Lemmas on the trace invariant ***)
+
+
+/// rephrasing of `trace_invariant` using `prefix_before_event`
+
+val prefix_before_event_invariant:
+  {|invs: protocol_invariants|} ->
+  ev:trace_event -> tr:trace{event_exists tr ev} ->
+  Lemma 
+    (requires trace_invariant tr)
+    (ensures trace_event_invariant (prefix_before_event ev tr) ev /\ trace_invariant (prefix_before_event ev tr))
+let rec prefix_before_event_invariant #invs the_ev tr = 
+  match tr with
+  | Nil -> ()
+  | Snoc init ev -> 
+         reveal_opaque (`%trace_invariant) (trace_invariant);
+         norm_spec [zeta; delta_only [`%trace_invariant]] (trace_invariant);
+         if ev = the_ev
+           then ()
+           else prefix_before_event_invariant the_ev init
 
 /// If there is an event in the trace satisfying the invariants,
 /// then this event satisfy the trace event invariant.
@@ -216,47 +268,47 @@ let msg_sent_on_network_are_publishable #invs tr msg =
     event_at_implies_trace_event_invariant tr i (MsgSent msg)
   )
 
+/// States stored satisfy the global state predicate.
+// only for the prefix right before the `SetState` event
+val state_was_set_implies_global_state_pred:
+  {|invs: protocol_invariants|} ->
+  p:principal -> sid:state_id -> content:state_raw -> tr:trace ->
+  Lemma
+    (requires 
+      trace_invariant tr
+      /\ state_was_set tr p sid content
+    )
+    (ensures
+      global_state_pred (prefix_before_event (SetState p sid content) tr) p sid content
+    )
+    [SMTPat (state_was_set tr p sid content); 
+     SMTPat (trace_invariant #invs tr);
+    ]
+let state_was_set_implies_global_state_pred p sid cont tr =
+  prefix_before_event_invariant (SetState p sid cont) tr
+
 /// States stored satisfy the custom state predicate.
-
-// val state_was_set_implies_pred:
-//   {|protocol_invariants|} -> tr:trace ->
-//   prin:principal -> sess_id:state_id -> content:bytes ->
-//   Lemma
-//   (requires
-//     trace_invariant tr /\
-//     state_was_set tr prin sess_id content
-//   )
-//   (ensures state_pred tr prin sess_id content)
-//   [SMTPat (state_was_set tr prin sess_id content);
-//    SMTPat (trace_invariant tr);
-//   ]
-// let state_was_set_implies_pred #invs tr prin sess_id content =
-//   eliminate exists i. event_at tr i (SetState prin sess_id content)
-//   returns invs.trace_invs.state_pred.pred tr prin sess_id content
-//   with _. (
-//     event_at_implies_trace_event_invariant tr i (SetState prin sess_id content);
-//     invs.trace_invs.state_pred.pred_later (prefix tr i) tr prin sess_id content
-//   )
-
+// together with `pred_later` this even holds for the complete trace
+// (as opposed to the prefix above)
 val state_was_set_implies_pred:
-  {|protocol_invariants|} -> tr:trace -> ts:timestamp ->
-  prin:principal -> sess_id:state_id -> content:bytes ->
+  {|invs: protocol_invariants|} -> tr:trace ->
+  prin:principal -> sess_id:state_id -> content:state_raw ->
   Lemma
   (requires
     trace_invariant tr /\
-    state_was_set_at tr ts prin sess_id content
+    state_was_set tr prin sess_id content
   )
-  (ensures state_pred (prefix tr ts) prin sess_id content)
-  [SMTPat (state_was_set_at tr ts prin sess_id content);
-   SMTPat (trace_invariant tr);
+  (ensures state_pred tr prin sess_id content)
+  [SMTPat (state_was_set tr prin sess_id content);
+   SMTPat (trace_invariant #invs tr);
   ]
-let state_was_set_implies_pred #invs tr ts prin sess_id content =
-  // eliminate exists i. event_at tr i (SetState prin sess_id content)
-  // returns invs.trace_invs.state_pred.pred tr prin sess_id content
-  // with _. (
-    event_at_implies_trace_event_invariant tr ts (SetState prin sess_id content)
-//    invs.trace_invs.state_pred.pred_later (prefix tr ts) tr prin sess_id content
-  // )
+let state_was_set_implies_pred #invs tr prin sess_id content =
+  eliminate exists i. event_at tr i (SetState prin sess_id content)
+  returns invs.trace_invs.state_pred.pred tr prin sess_id content
+  with _. (
+    event_at_implies_trace_event_invariant tr i (SetState prin sess_id content);
+    invs.trace_invs.state_pred.pred_later (prefix tr i) tr prin sess_id content
+  )
 
 
 /// States stored are knowable by the corresponding principal and state identifier.
@@ -264,7 +316,7 @@ let state_was_set_implies_pred #invs tr ts prin sess_id content =
 
 val state_is_knowable_by:
   {|protocol_invariants|} -> tr:trace ->
-  prin:principal -> sess_id:state_id -> content:bytes ->
+  prin:principal -> sess_id:state_id -> content:state_raw ->
   Lemma
   (requires
     trace_invariant tr /\
@@ -272,13 +324,12 @@ val state_is_knowable_by:
   )
   (ensures is_knowable_by (L.principal_state_label prin sess_id) tr content)
 let state_is_knowable_by #invs tr prin sess_id content =
- // state_was_set_lemma tr prin sess_id content;
   eliminate exists ts. event_at tr ts (SetState prin sess_id content)
   returns (is_knowable_by #invs.crypto_invs (L.principal_state_label prin sess_id) tr content)
   with _. (
     event_at_implies_trace_event_invariant tr ts (SetState prin sess_id content);
-   invs.trace_invs.state_pred.pred_later (prefix tr ts) tr prin sess_id content;
-  state_pred_knowable tr prin sess_id content
+    invs.trace_invs.state_pred.pred_later (prefix tr ts) tr prin sess_id content;
+    state_pred_knowable tr prin sess_id content
   )
   
 
