src/core/DY.Core.Trace.State.Aux.fst
@@ -5,17 +5,25 @@ open DY.Core.Bytes
 open DY.Core.Label.Type
 open DY.Core.Trace.Type
 
+/// This module defines helper functions for state handling on traces.
+/// The functions will be used in `DY.Core.Trace.Invariant`
+/// to define the trace invariant
+/// and in `DY.Core.Trace.Maniplation` where some are lifted to the `traceful` monad.
+
+
+/// Type aliases for the internal state layout
+/// 
 type state_raw = bytes
-type session_raw = rev_list state_raw
+type session_raw = rev_list state_raw // the current state of a session is the last entry
 type full_state_raw = list (state_id * session_raw) 
-//TODO: this should be `Map state_id session_raw`, can we extract the generic Map part from DY.Lib.State.Map?
+//TODO: full_state_raw should be `Map state_id session_raw`, can we extract the generic Map part from DY.Lib.State.Map?
 // or is it not worth the effort?
 
 val max: int -> int -> int
 let max x y =
   if x < y then y else x
 
-/// To add a new session to a state of a principal,
+/// To add a new session to a (full) state of a principal,
 /// we have to find a new identifier
 /// that is not used in the current state of the principal.
 
@@ -51,6 +59,8 @@ let rec compute_new_session_id_correct prin tr sess_id state_content =
     )
   )
 
+(*** Reading state, session, full state from the trace ***)
+
 val get_state_aux: principal -> state_id -> trace -> option state_raw
 let rec get_state_aux prin sess_id tr =
   match tr with
@@ -79,7 +89,8 @@ let get_session prin sess_id tr =
   match get_session_aux prin sess_id tr with
   | Nil -> None
   | sess -> Some sess
-  
+
+// simple tests to show intuition
 let _ =
   let p = "a" in
   let sid = {the_id = 1} in
@@ -88,6 +99,9 @@ let _ =
   assert(get_session p sid tr = Some (Snoc (Snoc Nil b) b));
   assert(None? (get_session "b" sid tr))
 
+
+/// Helper function for `get_full_state`
+ 
 val append_to: #a:eqtype -> #b:Type -> list (a * rev_list b) -> a -> b -> list (a * rev_list b)
 let append_to xys key elem =
   let (key_elems,rest) = FStar.List.Tot.Base.partition (fun (x, _) -> x = key) xys in
@@ -127,6 +141,7 @@ let get_full_state prin tr =
       | fst -> Some fst
     end
 
+// tests for `get_full_state`
 let _ =
   let p = "a" in
   let sid1 = {the_id = 1} in
@@ -136,6 +151,88 @@ let _ =
   assert(get_full_state p tr = Some [(sid1, (Snoc Nil b)); (sid2, Snoc Nil b)]);
   assert(None? (get_full_state "b" tr))
 
+
+(*** Properties for getter functions ***)
+
+
+val get_state_aux_state_was_set :
+  p:principal -> sid:state_id -> tr:trace ->
+  Lemma
+    (requires True)
+    (ensures (
+       match (get_state_aux p sid tr) with
+       | None -> True
+       | Some v -> state_was_set tr p sid v
+      )
+    )
+    [SMTPat (get_state_aux p sid tr)]
+let rec get_state_aux_state_was_set p sid tr =
+  match tr with
+  | Nil -> ()
+  | Snoc init (SetState p' sid' v) ->
+     if p' = p && sid' = sid 
+       then begin
+         let ev = (SetState p' sid' v) in
+         assert(event_at tr (DY.Core.Trace.Type.length tr - 1) ev)
+       end
+       else get_state_aux_state_was_set p sid init
+  | Snoc init _ -> get_state_aux_state_was_set p sid init
+
+val get_state_aux_is_last_of_get_session_aux:
+  p:principal -> sid:state_id -> tr:trace ->
+  Lemma 
+    (requires True
+    )
+    (ensures (
+      let session = get_session_aux p sid tr in
+      match get_state_aux p sid tr with
+      | None -> Nil? session
+      | Some st -> Snoc? session /\ (let Snoc _ last = session in st = last)
+    )
+    )
+let rec get_state_aux_is_last_of_get_session_aux p sid tr = 
+  match tr with
+  | Nil -> ()
+  | Snoc init _ -> get_state_aux_is_last_of_get_session_aux p sid init
+
+
+
+
+
+
+/// The main property we want to show is
+/// that a particular session of a principal stays the same
+/// if there are no more `SetState` entries for this principal and this session on the trace.
+
+/// The property that there are no state entries
+/// for the principal and a particular session
+
+val no_set_state_entry_for:
+  principal -> state_id -> trace -> prop
+let no_set_state_entry_for p sid tr = 
+  forall (ts:timestamp{ts < length tr}).
+    match get_event_at tr ts with
+    | SetState p' sid' _ -> p' <> p \/ sid' <> sid
+    | _ -> True
+
+/// if there are no state entries on a trace,
+/// this is true for any prefix of the trace.
+
+val no_set_state_entry_for_prefix:
+  p:principal -> sid:state_id -> tr1:trace -> tr2:trace ->
+  Lemma 
+    (requires no_set_state_entry_for p sid tr2 /\ tr1 <$ tr2)
+    (ensures no_set_state_entry_for p sid tr1)
+    [SMTPat (no_set_state_entry_for p sid tr2); SMTPat (tr1 <$ tr2)]
+let no_set_state_entry_for_prefix p sid tr1 tr2 = 
+  introduce forall (ts:timestamp{ts < length tr1}). get_event_at tr1 ts = get_event_at tr2 ts
+  with begin
+    let ev1 = get_event_at tr1 ts in
+    event_at_grows tr1 tr2 ts ev1
+    end
+
+/// definition of "trace substraction"
+/// (it holds: tr2 = tr1 ++ tr2 `suffix_after` tr1)
 
 val suffix_after: tr2:trace -> tr1:trace{tr1 <$ tr2} -> trace
 let rec suffix_after tr2 tr1 = 
@@ -150,20 +247,15 @@ let rec suffix_after tr2 tr1 =
              Snoc (suffix_after init tr1) ev
          end
 
-val no_set_state_entry_for:
-  principal -> state_id -> trace -> prop
-let no_set_state_entry_for p sid tr = 
-  forall (ts:timestamp{ts < DY.Core.Trace.Type.length tr}).
-    match get_event_at tr ts with
-    | SetState p' sid' _ -> p' <> p \/ sid' <> sid
-    | _ -> True
-
+/// for traces with tr1 <$ tr2 <$ tr3,
+/// the suffix after tr1 on tr2
+/// is a prefix of
+/// the suffix after tr1 on tr3
 
 val suffix_after_for_prefix: 
   tr3:trace -> tr2:trace {tr2 <$ tr3} -> tr1:trace {tr1 <$ tr2} ->
   Lemma 
-    (tr2 `suffix_after` tr1 <$ tr3 `suffix_after` tr1
-    )
+    (tr2 `suffix_after` tr1 <$ tr3 `suffix_after` tr1)
 let rec suffix_after_for_prefix tr3 tr2 tr1 = 
   reveal_opaque (`%grows) grows; 
   norm_spec [zeta; delta_only [`%prefix]] (prefix);
@@ -176,19 +268,9 @@ let rec suffix_after_for_prefix tr3 tr2 tr1 =
     end
 
 
-val no_set_state_entry_for_prefix:
-  p:principal -> sid:state_id -> tr1:trace -> tr2:trace ->
-  Lemma 
-    (requires no_set_state_entry_for p sid tr2 /\ tr1 <$ tr2)
-    (ensures no_set_state_entry_for p sid tr1)
-    [SMTPat (no_set_state_entry_for p sid tr2); SMTPat (tr1 <$ tr2)]
-let no_set_state_entry_for_prefix p sid tr1 tr2 = 
-  introduce forall (ts:timestamp{ts < DY.Core.Trace.Type.length tr1}). get_event_at tr1 ts = get_event_at tr2 ts
-  with begin
-    let ev1 = get_event_at tr1 ts in
-    event_at_grows tr1 tr2 ts ev1
-    end
-
+/// the main property:
+/// if there are no more state entries,
+/// the last state doesn't change
 
 val get_state_aux_same:
   p:principal -> sid:state_id -> tr1:trace -> tr2:trace ->
@@ -213,6 +295,7 @@ let rec get_state_aux_same p sid tr1 tr2 =
               get_state_aux_same p sid tr1 init
     end
 
+/// lifting of the get_state_aux property to get_session_aux
 
 val get_session_aux_same:
   p:principal -> sid:state_id -> tr1:trace -> tr2:trace ->
@@ -221,7 +304,6 @@ val get_session_aux_same:
       tr1 <$ tr2 /\ no_set_state_entry_for p sid (tr2 `suffix_after` tr1)
     )
     (ensures get_session_aux p sid tr1 = get_session_aux p sid tr2)
- //   [SMTPat (tr1 <$ tr2 /\ no_set_state_entry_for p sid (tr2 `suffix_after` tr1))]
 let rec get_session_aux_same p sid tr1 tr2 =
   reveal_opaque (`%grows) grows; 
   norm_spec [zeta; delta_only [`%prefix]] (prefix);
